use IntSeq for bignum

specs/experimental/Spec.Bignum.LL.Lib.fst
@@ -1,108 +1,84 @@
 module Spec.Bignum.LL.Lib
 
-open FStar.Seq
 open FStar.Mul
-open FStar.UInt
 open FStar.Math.Lemmas
-open Spec.Seq.Lib
-open Spec.Bignum.Lib
 
-module U32 = FStar.UInt32
-module U64 = FStar.UInt64
-module U128 = FStar.UInt128
-open U32
+open Spec.Lib.IntTypes
+open Spec.Lib.RawIntTypes
+open Spec.Lib.IntSeq
+open Spec.Lib.IntSeq.Lemmas
 
 type bignum = nat
-type seqbn = Spec.Seq.Lib.seq U64.t
-type lseqbn len = s:seqbn{length s = U32.v len}
-type carry = U64.t //c:U64.t{U64.v c = 1 \/ U64.v c = 0}
 
-let x_i i = pow2 (64 * v i)
+type lseqbn len = intseq U64 len
+type carry = uint64
 
-val eval_i: s:seqbn -> i:U32.t{v i <= length s} -> Tot bignum (decreases (v i))
-let rec eval_i s i =
-    if i =^ 0ul then 0
-    else eval_i s (i -^ 1ul) + U64.v s.[i -^ 1ul] * x_i (i -^ 1ul)
+let x_i (i:size_nat) = pow2 (64 * i)
 
-val eval: s:seqbn -> Tot bignum
-let eval s = eval_i s (seq_length s)
+val eval_i:
+    len:size_nat{len > 0} -> s:lseqbn len -> i:size_nat{i <= len} -> Tot bignum (decreases i)
+let rec eval_i len s i =
+    if i = 0 then 0
+    else eval_i len s (i - 1) + (uint_to_nat s.[i - 1]) * x_i (i - 1)
 
-val lemma_eval_incr: s:seqbn -> i:U32.t{0 < v i /\ v i <= length s} -> Lemma
+val eval:
+    len:size_nat{len > 0} -> s:lseqbn len -> Tot bignum
+let eval len s = eval_i len s len
+
+val lemma_eval_i:
+    len:size_nat -> s1:lseqbn len -> s2:lseqbn len -> i:size_nat{i < len} -> Lemma
+    (requires (forall (j:size_nat). j < i ==> s1.[j] == s2.[j]))
+    (ensures (eval_i len s1 i == eval_i len s2 i))
+    (decreases i)
+let rec lemma_eval_i len s1 s2 i =
+    if i = 0 then ()
+    else lemma_eval_i len s1 s2 (i - 1)
+
+val lemma_eval_incr:
+    len:size_nat{len > 0} ->  s:lseqbn len -> i:size_nat{0 < i /\ i <= len} -> Lemma
     (requires (True))
-    (ensures (eval_i s i = eval_i s (i -^ 1ul) + U64.v s.[i -^ 1ul] * x_i (i -^ 1ul)))
-let lemma_eval_incr s i = ()
+    (ensures (eval_i len s i == eval_i len s (i - 1) + (uint_to_nat s.[i - 1]) * x_i (i - 1)))
+let rec lemma_eval_incr len s i = ()
 
-val lemma_mult_x1_xi1: i:U32.t{v i > 0} -> x1:nat -> xi1:nat -> Lemma
-    (requires (x1 = x_i 1ul /\ xi1 = x_i (i -^ 1ul)))
+val lemma_eval_init_seq_is_0: 
+    len:size_nat{len > 0} -> s:lseqbn len -> i:size_nat{i <= len} -> Lemma
+    (requires (forall (j:size_nat). j < len ==> uint_to_nat s.[j] = 0))
+    (ensures (eval_i len s i = 0))
+    (decreases i)
+
+#reset-options "--z3rlimit 50 --max_fuel 2"
+
+let rec lemma_eval_init_seq_is_0 len s i =
+    if i = 0 then ()
+    else lemma_eval_init_seq_is_0 len s (i - 1)
+
+val lemma_mult_x1_xi1:
+    i:size_nat{i > 0} -> x1:nat -> xi1:nat -> Lemma
+    (requires (x1 = x_i 1 /\ xi1 = x_i (i - 1)))
     (ensures (x1 * xi1 = x_i i))
 let lemma_mult_x1_xi1 i x1 xi =
-    pow2_plus (64 * U32.v 1ul) (64 * U32.v (i -^ 1ul));
-    assert (pow2 (64 * U32.v 1ul) * pow2 (64 * U32.v (i -^ 1ul)) = pow2 ((64 * U32.v 1ul) + (64 * U32.v (i -^ 1ul))));
-    assert (pow2 (64 * U32.v 1ul) * pow2 (64 * U32.v (i -^ 1ul)) = pow2 (64 * U32.v i))
+    pow2_plus (64 * 1) (64 * (i - 1));
+    assert (pow2 (64 * 1) * pow2 (64 * (i - 1)) = pow2 (64 * 1 + 64 * (i - 1)));
+    assert (pow2 (64 * 1) * pow2 (64 * (i - 1)) = pow2 (64 * i))
 
-val lemma_mult_xi_xj: i:U32.t -> j:U32.t -> xi:nat -> xj:nat -> Lemma
-    (requires (xi = x_i i /\ xj = x_i j /\ v i + v j < pow2 32))
-    (ensures (v i + v j < pow2 32 /\ xi * xj = x_i (i +^ j)))
+val lemma_mult_xi_xj:
+    i:size_nat -> j:size_nat -> xi:nat -> xj:nat -> Lemma
+    (requires (xi = x_i i /\ xj = x_i j /\ i + j < max_size_t))
+    (ensures (i + j < max_size_t /\ xi * xj = x_i (i + j)))
 let lemma_mult_xi_xj i j xi xj =
-    pow2_plus (64 * U32.v i) (64 * U32.v j)
+    pow2_plus (64 * i) (64 * j)
 
-val lemma_upd: len:U32.t -> s:lseqbn len -> s':lseqbn len -> i1:U32.t{U32.v i1 < U32.v len} -> s_i1:U64.t -> Lemma
-    (requires (s' = (s.[i1] <- s_i1)))
-    (ensures (forall i. (i <> v i1 /\ i < v len) ==> s.[uint_to_t i] = s'.[uint_to_t i]))
-let lemma_upd len s s' i1 s_i1 = ()
+val lemma_mul_assoc:
+    a:nat -> b:nat -> c:nat -> Lemma
+    (a * b * c = a * (b * c))
+let lemma_mul_assoc a b c = ()
 
-val lemma_eval_i: len:U32.t -> s1:lseqbn len -> s2:lseqbn len -> i:U32.t{v i < v len} -> Lemma
-    (requires (forall j. v j  <  v i ==> s1.[j] == s2.[j]))
-    (ensures (eval_i s1 i == eval_i s2 i))
-    (decreases (v i))
-let rec lemma_eval_i len s1 s2 i =
-    if i =^ 0ul then ()
-    else lemma_eval_i len s1 s2 (i -^ 1ul)
-
-#reset-options "--z3rlimit 30 --max_fuel 0"
-
-val lemma_eval_upd: len:U32.t -> s:lseqbn len -> i1:U32.t{v i1 < length s} -> s_i1:U64.t -> Lemma
-    (requires (True))
-    (ensures (let s' = s.[i1] <- s_i1 in eval_i s i1 == eval_i s' i1))
-let lemma_eval_upd len s i1 s_i1 =
-    let s' = s.[i1] <- s_i1 in
-    lemma_upd len s s' i1 s_i1;
-    assert (slice s 0ul i1 == slice s' 0ul i1);
-    lemma_eval_i len s s' i1;
-    assert (eval_i s i1 == eval_i s' i1)
-
-#reset-options "--z3rlimit 30 --max_fuel 2"
-
-val lemma_eval_init_seq_is_0: len:U32.t -> s:lseqbn len -> i:U32.t{v i <= v len} -> Lemma
-    (requires (forall j. v j < v len ==> s.[j] = 0uL))
-    (ensures (eval_i s i = 0))
-    (decreases (v i))
-let rec lemma_eval_init_seq_is_0 len s i =
-    if i =^ 0ul then ()
-    else lemma_eval_init_seq_is_0 len s (i -^ 1ul)
-
-#reset-options 
-
-val lemma_distributivity_add_fold: a:int -> b:int -> c:int -> Lemma
-  (a * b + a * c = a * (b + c))
-let lemma_distributivity_add_fold a b c = ()
-
-val lemma_distributivity_add_fold_right: a:int -> b:int -> c:int -> Lemma
-  (b * a + c * a = (b + c) * a)
-let lemma_distributivity_add_fold_right a b c = ()
-
-val lemma_distributivity_add_add_sub: a:int -> b:int -> c:int -> d:int -> e:int -> Lemma
+val lemma_distributivity_add_add_sub: 
+  a:nat -> b:nat -> c:nat -> d:nat -> e:nat -> Lemma
   ((a + b + c - d) * e = a * e + b * e + c * e - d * e)
 let lemma_distributivity_add_add_sub a b c d e = ()
 
-#reset-options "--z3rlimit 50 --max_fuel 0"
-
-val lemma_mult_add_add_64: a:U64.t -> b:U64.t -> c:U64.t -> d:U64.t -> Lemma
-    (U64.v a * U64.v b + U64.v c + U64.v d < pow2 128)
-
-let lemma_mult_add_add_64 a b c d =
-    let n = pow2 64 in
-    assert (U64.v a <= n - 1 /\ U64.v b <= n - 1 /\ U64.v c <= n - 1 /\ U64.v d <= n - 1);
-    assert (U64.v a * U64.v b + U64.v c + U64.v d <= (n - 1) * (n - 1) + (n - 1) + (n - 1));
-    assert ((n - 1) * (n - 1) + (n - 1) + (n - 1) == n * n - 1);
-    pow2_plus 64 64
+val lemma_distributivity_add_fold: 
+  a:nat -> b:nat -> c:nat -> Lemma
+  (a * b + a * c = a * (b + c))
+let lemma_distributivity_add_fold a b c = ()
