specs/experimental/Spec.Bignum.LL.fst
@@ -1,209 +1,217 @@
 module Spec.Bignum.LL
 
-open FStar.Seq
 open FStar.Mul
-open FStar.UInt
 open FStar.Math.Lemmas
-open Spec.Seq.Lib
-open Spec.Bignum.Lib
+
+open Spec.Lib.IntTypes
+open Spec.Lib.RawIntTypes
+open Spec.Lib.IntSeq
+open Spec.Lib.IntSeq.Lemmas
 open Spec.Bignum.LL.Lib
 
-module U32 = FStar.UInt32
-module U64 = FStar.UInt64
-module U128 = FStar.UInt128
-open U32
-
-(*
-#reset-options "--z3rlimit 150 --max_fuel 0"
-
-val add_with_carry: a:U64.t -> b:U64.t -> c:carry -> Pure (tuple2 carry U64.t)
+(* ADDITION *)
+val add_with_carry:
+    a:uint64 -> b:uint64 -> c:carry -> Pure (tuple2 carry uint64)
     (requires (True))
-    (ensures (fun (c', r) -> U64.v r + U64.v c' * x_i 1ul = U64.v a + U64.v b + U64.v c))
-
-let add_with_carry a b c =
-    let r = U64.(a +%^ b +%^ c) in
-    assert (U64.v r = (U64.v a + U64.v b + U64.v c) % pow2 64);
-    let (c', r) = if U64.(r <^ a) then (1uL, r) else (0uL, r) in
-    assume (U64.v c' = (U64.v a + U64.v b + U64.v c) / pow2 64);
-    lemma_div_mod (U64.v a + U64.v b + U64.v c) (pow2 64);
-    assert (x_i 1ul = pow2 64);
-    (c', r)
-
-#reset-options "--z3rlimit 150 --max_fuel 2"
-
-val sum_:
-    len:U32.t -> a:lseqbn len -> b:lseqbn len ->
-    i:U32.t{v i <= v len} -> res:lseqbn len -> Pure (tuple2 carry (lseqbn len))
-    (requires (True))
-    (ensures (fun (c', res') -> eval_i res' i + U64.v c' * x_i i == eval_i a i + eval_i b i))
-    (decreases (v i))
-
-let rec sum_ len a b i res =
-    if i =^ 0ul then
-       (0uL, res)
-    else begin
-        let i1 = i -^ 1ul in
-        let (c, r) = sum_ len a b i1 res in
-        assert (eval_i r i1 + U64.v c * x_i i1 == eval_i a i1 + eval_i b i1); // from rec ind hypo
-        let (c', res_i) = add_with_carry a.[i1] b.[i1] c in
-        assert (U64.v res_i + U64.v c' * x_i 1ul == U64.v a.[i1] + U64.v b.[i1] + U64.v c); // from add_with_carry
-        let res' = r.[i1] <- res_i in
-        lemma_eval_upd len r i1 res_i;
-        assert (eval_i res' i1 == eval_i r i1); // from upd
-        assert (eval_i res' i == eval_i res' i1 + U64.v res'.[i1] * x_i i1); //from eval_i
-        assert (eval_i res' i == eval_i a i1 + eval_i b i1 - U64.v c * x_i i1 + (U64.v a.[i1] + U64.v b.[i1] + U64.v c - U64.v c' * x_i 1ul) * x_i i1); //expansion
-        assert (eval_i res' i == eval_i a i1 + eval_i b i1 - U64.v c * x_i i1 + U64.v a.[i1] * x_i i1  + U64.v b.[i1] * x_i i1  + U64.v c * x_i i1  - U64.v c' * x_i 1ul * x_i i1);
-        assert (eval_i res' i == eval_i a i1 + eval_i b i1 + U64.v a.[i1] * x_i i1  + U64.v b.[i1] * x_i i1  - U64.v c' * x_i 1ul * x_i i1);
-        assert (eval_i res' i + U64.v c' * x_i 1ul * x_i i1  == eval_i a i + eval_i b i);
-        lemma_mult_x1_xi1 i (x_i 1ul) (x_i i1);
-        (c', res')
-    end
-
-val sum: 
-    len:U32.t -> a:lseqbn len -> b:lseqbn len -> Pure (tuple2 carry (lseqbn len))
-    (requires (True))
-    (ensures (fun (c', res') -> eval_i res' len + U64.v c' * x_i len = eval_i a len + eval_i b len))
-let sum len a b =
-    let res = create len 0uL in
-    sum_ len a b len res
-*)
+    (ensures (fun (c', r) -> uint_v r + uint_v c' * x_i 1 = uint_v a + uint_v b + uint_v c))
 
 #reset-options "--z3rlimit 50 --max_fuel 0"
 
-val mult_by_limb_addj_f:
-    a_i:U64.t -> l:U64.t -> c:U64.t -> r_ij:U64.t -> Pure (tuple2 carry U64.t)
-    (requires (True))
-    (ensures (fun (c', r) -> U64.v r + U64.v c' * x_i 1ul == U64.v a_i * U64.v l + U64.v c + U64.v r_ij))
-
-let mult_by_limb_addj_f a_i l c r_ij =
-    lemma_mult_add_add_64 a_i l c r_ij;
-    let res = U128.(mul_wide a_i l +^ uint64_to_uint128 c +^ uint64_to_uint128 r_ij) in
-    let r = U128.uint128_to_uint64 res in
-    let c' = U128.shift_right res 64ul in
-    let c' = U128.uint128_to_uint64 c' in
-    lemma_div_mod (U64.v a_i * U64.v l + U64.v c + U64.v r_ij) (pow2 64);
+let add_with_carry a b c =
+    let tmp = to_u128 a +! to_u128 b +! to_u128 c in
+    let r = to_u64 tmp in
+    assert (uint_v r = (uint_v a + uint_v b + uint_v c) % pow2 64);
+    let c' = to_u64 (tmp >>. (u32 64)) in
+    assert (uint_v c' = (uint_v a + uint_v b + uint_v c) / pow2 64);
+    lemma_div_mod (uint_v a + uint_v b + uint_v c) (pow2 64);
+    assert_norm (x_i 1 = pow2 64);
     (c', r)
 
-#reset-options "--z3rlimit 300 --max_fuel 0"
+val sum_:
+    len:size_nat{len > 0} -> a:lseqbn len -> b:lseqbn len ->
+    i:size_nat{i <= len} -> res:lseqbn len -> Pure (tuple2 carry (lseqbn len))
+    (requires (True))
+    (ensures (fun (c', res') -> eval_i len res' i + uint_v c' * x_i i == eval_i len a i + eval_i len b i))
+    (decreases i)
+
+#reset-options "--z3rlimit 150 --max_fuel 2"
+
+let rec sum_ len a b i res =
+    if i = 0 then
+       (u64 0, res)
+    else begin
+        let i1 = i - 1 in
+        let (c, r) = sum_ len a b i1 res in
+        //assert (eval_i len r i1 + uint_v #U64 c * x_i i1 == eval_i len a i1 + eval_i len b i1); // from rec ind hypo
+        let (c', res_i) = add_with_carry a.[i1] b.[i1] c in
+        //assert (uint_v #U64 res_i + uint_v #U64 c' * x_i 1 == uint_v #U64 a.[i1] + uint_v #U64 b.[i1] + uint_v #U64 c); // from add_with_carry
+        let res' = r.[i1] <- res_i in
+        lemma_eval_i len r res' i1;
+        //assert (eval_i len res' i1 == eval_i len r i1); // from upd
+        assert (eval_i len res' i == eval_i len res' i1 + (uint_v res'.[i1]) * x_i i1); //from eval_i
+        assert (eval_i len res' i == eval_i len a i1 + eval_i len b i1 - uint_v c * x_i i1 + (uint_v a.[i1] + uint_v b.[i1] + uint_v c - uint_v c' * x_i 1) * x_i i1); //expansion
+        assert (eval_i len res' i == eval_i len a i1 + eval_i len b i1 - uint_v c * x_i i1 + uint_v a.[i1] * x_i i1  + uint_v b.[i1] * x_i i1  + uint_v c * x_i i1  - uint_v c' * x_i 1 * x_i i1);
+        assert (eval_i len res' i == eval_i len a i1 + eval_i len b i1 + uint_v a.[i1] * x_i i1  + uint_v b.[i1] * x_i i1  - uint_v c' * x_i 1 * x_i i1);
+        assert (eval_i len res' i + uint_v c' * x_i 1 * x_i i1  == eval_i len a i + eval_i len b i);
+	lemma_mul_assoc (uint_v c') (x_i 1) (x_i i1);
+        lemma_mult_x1_xi1 i (x_i 1) (x_i i1);
+	assert (eval_i len res' i + uint_v c' * x_i i  == eval_i len a i + eval_i len b i);
+        (c', res')
+    end
+
+val sum:
+    len:size_nat{len > 0} -> a:lseqbn len -> b:lseqbn len -> Pure (tuple2 carry (lseqbn len))
+    (requires (True))
+    (ensures (fun (c', res') -> eval_i len res' len + uint_v c' * x_i len = eval_i len a len + eval_i len b len))
+    
+let sum len a b =
+    let res = create len (u64 0) in
+    sum_ len a b len res
+
+(* MULTIPLICATION *)
+
+val lemma_mult_add_add_64: 
+    a:uint64 -> b:uint64 -> c:uint64 -> d:uint64 -> Lemma
+    (uint_v a * uint_v b + uint_v c + uint_v d < pow2 128)
+
+#reset-options "--z3rlimit 50 --max_fuel 0 --max_ifuel 0"
+
+let lemma_mult_add_add_64 a b c d =
+    let n = pow2 64 in
+    assert (uint_v a <= n - 1 /\ uint_v b <= n - 1 /\ uint_v c <= n - 1 /\ uint_v d <= n - 1);
+    assert (uint_v a * uint_v b + uint_v c + uint_v d <= (n - 1) * (n - 1) + (n - 1) + (n - 1));
+    assert ((n - 1) * (n - 1) + (n - 1) + (n - 1) == n * n - 1);
+    pow2_plus 64 64
+
+assume val mult_by_limb_addj_f:
+    a_i:uint64 -> l:uint64 -> c:uint64 -> r_ij:uint64 -> Pure (tuple2 carry uint64)
+    (requires (True))
+    (ensures (fun (c', r) -> uint_v r + uint_v c' * x_i 1 == uint_v a_i * uint_v l + uint_v c + uint_v r_ij))
+
+(*
+let mult_by_limb_addj_f a_i l c r_ij =
+    lemma_mult_add_add_64 a_i l c r_ij;
+    //let res = mul_wide a_i l +! to_u128 c +! to_u128 r_ij in
+    let res = to_u128 c +! to_u128 r_ij in
+    let r = to_u64 res in
+    let c' = res >>. u32 64 in
+    let c' = to_u64 c' in
+    lemma_div_mod (uint_v a_i * uint_v l + uint_v c + uint_v r_ij) (pow2 64);
+    (c', r)
+*)
 
 (* (forall k. (v i1 + v j <= k /\ k < v resLen) ==> res.[uint_to_t k] = r1.[uint_to_t k]) *)
 val mult_by_limb_addj_inner:
-    len:U32.t -> a:lseqbn len -> l:U64.t -> i1:U32.t{v i1 < v len} ->
-    j:U32.t -> resLen:U32.t{v len + v j < v resLen} ->
-    res:lseqbn resLen -> c1:carry -> r1:lseqbn resLen ->
-    Pure (tuple2 carry (lseqbn resLen))
-    (requires (eval_i r1 (i1 +^ j) + U64.v c1 * x_i (i1 +^ j) == eval_i res (i1 +^ j) + eval_i a i1 * U64.v l * x_i j /\
-               res.[i1 +^ j] = r1.[i1 +^ j]))
-    (ensures (fun (c', res') -> let i = i1 +^ 1ul in
-        eval_i res' (i +^ j) + U64.v c' * x_i (i +^ j) == eval_i res (i +^ j) + eval_i a i * U64.v l * x_i j))
+    len:size_nat -> a:lseqbn len -> l:uint64 -> i1:size_nat{i1 < len} ->
+    j:size_nat -> resLen:size_nat{len + j < resLen} ->
+    res:lseqbn resLen -> c1:carry -> r1:lseqbn resLen -> Pure (tuple2 carry (lseqbn resLen))
+    (requires (eval_i resLen r1 (i1 + j) + uint_v c1 * x_i (i1 + j) == eval_i resLen res (i1 + j) + eval_i len a i1 * uint_v l * x_i j /\ 
+	      uint_v res.[i1 + j] = uint_v r1.[i1 + j]))
+    (ensures (fun (c', res') -> let i = i1 + 1 in
+	      eval_i resLen res' (i + j) + uint_v c' * x_i (i + j) == eval_i resLen res (i + j) + eval_i len a i * uint_v l * x_i j))
+
+#reset-options "--z3rlimit 150 --max_fuel 0"
 
 let mult_by_limb_addj_inner len a l i1 j resLen res c1 r1 =
-    let i = i1 +^ 1ul in
-    let (c', res_ij) = mult_by_limb_addj_f a.[i1] l c1 r1.[i1 +^ j] in
-    let res' = r1.[i1 +^ j] <- res_ij in
-    lemma_eval_upd resLen r1 (i1 +^ j) res_ij;
-    lemma_eval_incr res' (i +^ j);
-    assert (eval_i res' (i +^ j) == eval_i res' (i +^ j -^ 1ul) + U64.v res'.[i +^ j -^ 1ul] * x_i (i +^ j -^ 1ul));
-    assert (eval_i res' (i +^ j) ==
-            eval_i res (i1 +^ j) + eval_i a i1 * U64.v l * x_i j - U64.v c1 * x_i (i1 +^ j) +
-            (U64.v a.[i1] * U64.v l + U64.v c1 + U64.v r1.[i1 +^ j] - U64.v c' * x_i 1ul) * x_i (i1 +^ j));
-    lemma_distributivity_add_add_sub (U64.v a.[i1] * U64.v l) (U64.v c1) (U64.v r1.[i1 +^ j]) (U64.v c' * x_i 1ul) (x_i (i1 +^ j));
-    lemma_mult_x1_xi1 (i +^ j) (x_i 1ul) (x_i (i1 +^ j));
-    assert (eval_i res' (i +^ j) + U64.v c' * x_i (i +^ j) ==
-            eval_i res (i1 +^ j) + eval_i a i1 * U64.v l * x_i j + U64.v a.[i1] * U64.v l * x_i (i1 +^ j) +
-            U64.v r1.[i1 +^ j] * x_i (i1 +^ j));
-    assert (res.[i1 +^ j] = r1.[i1 +^ j]);
-    lemma_eval_incr res (i +^ j);
+    let i = i1 + 1 in
+    let (c', res_ij) = mult_by_limb_addj_f a.[i1] l c1 r1.[i1 + j] in
+    assert (uint_v res_ij + uint_v c' * x_i 1 == uint_v a.[i1] * uint_v l + uint_v c1 + uint_v r1.[i1 + j]);
+    let res' = r1.[i1 + j] <- res_ij in
+    lemma_eval_i resLen r1 res' (i1 + j);
+    lemma_eval_incr resLen res' (i + j);
+    assert (eval_i resLen res' (i + j) == eval_i resLen res' (i + j - 1) + uint_v res'.[i + j - 1] * x_i (i + j - 1));
+    assert (eval_i resLen res' (i1 + j) == eval_i resLen r1 (i1 + j));
+    assert (eval_i resLen res' (i + j) == eval_i resLen res (i1 + j) + eval_i len a i1 * uint_v l * x_i j - uint_v c1 * x_i (i1 + j) +
+            (uint_v a.[i1] * uint_v l + uint_v c1 + uint_v r1.[i1 + j] - uint_v c' * x_i 1) * x_i (i1 + j));
+    lemma_distributivity_add_add_sub (uint_v a.[i1] * uint_v l) (uint_v c1) (uint_v r1.[i1 + j]) (uint_v c' * x_i 1) (x_i (i1 + j));
+    lemma_mult_x1_xi1 (i + j) (x_i 1) (x_i (i1 + j));
+    assert (eval_i resLen res' (i + j) + uint_v c' * x_i (i + j) == 
+            eval_i resLen res (i1 + j) + eval_i len a i1 * uint_v l * x_i j + uint_v a.[i1] * uint_v l * x_i (i1 + j) + uint_v r1.[i1 + j] * x_i (i1 + j));
+    lemma_eval_incr resLen res (i + j);
     lemma_mult_xi_xj i1 j (x_i i1) (x_i j);
-    lemma_distributivity_add_fold_right (U64.v l * x_i j) (eval_i a i1) (U64.v a.[i1] * x_i i1);
-    lemma_eval_incr a i;
+    lemma_eval_incr len a i;
     (c', res')
-
-#reset-options "--z3rlimit 50 --max_fuel 2"
 
 //(forall k. (v i + v j <= k /\ k < v resLen) ==> res.[uint_to_t k] = res'.[uint_to_t k])
 val mult_by_limb_addj_:
-    len:U32.t -> a:lseqbn len -> l:U64.t -> i:U32.t{v i <= v len} ->
-    j:U32.t -> resLen:U32.t{v len + v j < v resLen} ->
+    len:size_nat{len > 0} -> a:lseqbn len -> l:uint64 -> i:size_nat{i <= len} ->
+    j:size_nat -> resLen:size_nat{len + j < resLen} ->
     res:lseqbn resLen -> Pure (tuple2 carry (lseqbn resLen))
     (requires (True))
-    (ensures (fun (c', res') -> eval_i res' (i +^ j) + U64.v c' * x_i (i +^ j) ==
-                                eval_i res (i +^ j) + eval_i a i * U64.v l * x_i j /\ 
-                                (forall k. (v i + v j <= k /\ k < v resLen) ==> res.[uint_to_t k] = res'.[uint_to_t k])))
-    (decreases (v i))
+    (ensures (fun (c', res') -> eval_i resLen res' (i + j) + uint_v c' * x_i (i + j) == eval_i resLen res (i + j) + eval_i len a i * uint_v l * x_i j /\
+                             (forall k. (i + j <= k /\ k < resLen) ==> uint_v res.[k] = uint_v res'.[k])))
+    (decreases i)
+
+#reset-options "--z3rlimit 100 --max_fuel 2"
 
 let rec mult_by_limb_addj_ len a l i j resLen res =
-    if i =^ 0ul then
-        (0uL, res)
+    if i = 0 then
+        (u64 0, res)
     else begin
-        let i1 = i -^ 1ul in
+        let i1 = i - 1 in
         let (c1, r1) = mult_by_limb_addj_ len a l i1 j resLen res in
-        assert (res.[i1 +^ j] = r1.[i1 +^ j]); //from ind hypo
+        assert (uint_v res.[i1 + j] = uint_v r1.[i1 + j]); //from ind hypo
         let (c', res') = mult_by_limb_addj_inner len a l i1 j resLen res c1 r1 in
         (c', res')
     end
 
-#reset-options
-
 val mult_by_limb_addj:
-    len:U32.t -> a:lseqbn len -> l:U64.t -> j:U32.t ->
-    resLen:U32.t{v len + v j < v resLen} ->
+    len:size_nat{len > 0} -> a:lseqbn len -> l:uint64 -> j:size_nat ->
+    resLen:size_nat{len + j < resLen} ->
     res:lseqbn resLen -> Pure (tuple2 carry (lseqbn resLen))
     (requires (True))
-    (ensures (fun (c', res') -> eval_i res' (len +^ j) + U64.v c' * x_i (len +^ j) ==
-                                eval_i res (len +^ j) + eval a * U64.v l * x_i j))
+    (ensures (fun (c', res') -> eval_i resLen res' (len + j) + uint_v c' * x_i (len + j) == eval_i resLen res (len + j) + eval len a * uint_v l * x_i j))
 
 let mult_by_limb_addj len a l j resLen res = mult_by_limb_addj_ len a l len j resLen res
 
-#reset-options "--z3rlimit 300 --max_fuel 0"
 
 val mult_inner:
-    len:U32.t -> a:lseqbn len -> b:lseqbn len ->
-    resLen:U32.t{v resLen = v len + v len} ->
-    j1:U32.t{v j1 < v len} -> r:lseqbn resLen -> Pure (lseqbn resLen)
-    (requires (eval_i r (len +^ j1) == eval a * eval_i b j1))
-    (ensures (fun res' -> let j = j1 +^ 1ul in
-        eval_i res' (len +^ j) == eval a * eval_i b j))
+    len:size_nat -> a:lseqbn len -> b:lseqbn len ->
+    resLen:size_nat{resLen = len + len} ->
+    j1:size_nat{j1 < len} -> r:lseqbn resLen -> Pure (lseqbn resLen)
+    (requires (eval_i resLen r (len + j1) == eval len a * eval_i len b j1))
+    (ensures (fun res' -> let j = j1 + 1 in
+        eval_i resLen res' (len + j) == eval len a * eval_i len b j))
+
+#reset-options "--z3rlimit 300 --max_fuel 0"
 
 let mult_inner len a b resLen j1 r =
-    let j = j1 +^ 1ul in
+    let j = j1 + 1 in
+    assert (eval_i resLen r (len + j1) + eval len a * uint_v b.[j1] * x_i j1 == eval len a * eval_i len b j1 + eval len a * uint_v b.[j1] * x_i j1);
+    lemma_distributivity_add_fold (eval len a) (eval_i len b j1) (uint_v b.[j1] * x_i j1);
+    lemma_eval_incr len b j;
+    assert (eval_i resLen r (len + j1) + eval len a * uint_v b.[j1] * x_i j1 == eval len a * eval_i len b j);
+    
     let (c', res') = mult_by_limb_addj len a b.[j1] j1 resLen r in
-    assert (eval_i r (len +^ j1) + eval a * U64.v b.[j1] * x_i j1 ==
-            eval a * eval_i b j1 + eval a * U64.v b.[j1] * x_i j1);
-    lemma_distributivity_add_fold (eval a) (eval_i b j1) (U64.v b.[j1] * x_i j1);
-    lemma_eval_incr b j;
-    assert (eval_i res' (len +^ j1) + U64.v c' * x_i (len +^ j1) == eval a * eval_i b j);
-    let res1 = res'.[len +^ j1] <- c' in
-    lemma_eval_upd resLen res' (len +^ j1) c';
-    lemma_eval_incr res1 (len +^ j);
-    assert (eval_i res1 (len +^ j) == eval a * eval_i b j);
+    assert (eval_i resLen res' (len + j1) + uint_v c' * x_i (len + j1) == eval len a * eval_i len b j);
+    let res1 = res'.[len + j1] <- c' in
+    lemma_eval_i resLen res' res1 (len + j1);
+    lemma_eval_incr resLen res1 (len + j);
+    assert (eval_i resLen res1 (len + j) == eval len a * eval_i len b j);
     res1
+
+val mult_:
+    len:size_nat{len > 0} -> a:lseqbn len -> b:lseqbn len ->
+    resLen:size_nat{resLen = len + len} ->
+    j:size_nat{j <= len} -> Tot (res':lseqbn resLen{eval_i resLen res' (len + j) == eval len a * eval_i len b j})
+    (decreases j)
 
 #reset-options "--z3rlimit 50 --max_fuel 2"
 
-val mult_:
-    len:U32.t -> a:lseqbn len -> b:lseqbn len ->
-    resLen:U32.t{v resLen = v len + v len} ->
-    j:U32.t{v j <= v len} -> Tot (res':lseqbn resLen{eval_i res' (len +^ j) == eval a * eval_i b j})
-    (decreases (v j))
-
 let rec mult_ len a b resLen j  =
-    if j =^ 0ul then begin
-        let res' = create resLen 0uL in
-        lemma_eval_init_seq_is_0 resLen res' (len +^ j);
-        res'
-        end
+    if j = 0 then begin
+        let res' = create resLen (u64 0) in
+        lemma_eval_init_seq_is_0 resLen res' (len + j);
+        res' end
     else begin
-        let j1 = j -^ 1ul in
+        let j1 = j - 1 in
         let r = mult_ len a b resLen j1 in
         mult_inner len a b resLen j1 r 
     end
 
-#reset-options
-
 val mult:
-    len:U32.t -> a:lseqbn len -> b:lseqbn len ->
-    resLen:U32.t{v resLen = v len + v len} ->
-    Tot (res':lseqbn resLen{eval res' == eval a * eval b})
+    len:size_nat{len > 0} -> a:lseqbn len -> b:lseqbn len ->
+    resLen:size_nat{resLen = len + len} ->
+    Tot (res':lseqbn resLen{eval resLen res' == eval len a * eval len b})
 
 let mult len a b resLen = mult_ len a b resLen len
